@prefix : <https://www.w3.org/2019/wot/tm#> .
@prefix dc: <http://purl.org/dc/elements/1.1/> .
@prefix owl: <http://www.w3.org/2002/07/owl#> .
@prefix rdf: <http://www.w3.org/1999/02/22-rdf-syntax-ns#> .
@prefix xml: <http://www.w3.org/XML/1998/namespace> .
@prefix xsd: <http://www.w3.org/2001/XMLSchema#> .
@prefix foaf: <http://xmlns.com/foaf/0.1/> .
@prefix rdfs: <http://www.w3.org/2000/01/rdf-schema#> .
@prefix vann: <http://purl.org/vocab/vann/> .
@prefix dcterms: <http://purl.org/dc/terms/> .
@prefix schema: <http://schema.org/> .
@prefix hctl: <https://www.w3.org/2019/wot/hypermedia#> .
@prefix tm: <https://www.w3.org/2019/wot/tm#> .


dc:title a owl:AnnotationProperty .
vann:preferredNamespacePrefix a owl:AnnotationProperty .
vann:preferredNamespaceUri a owl:AnnotationProperty .
dcterms:description a owl:AnnotationProperty .
dcterms:license a owl:AnnotationProperty .
dcterms:contributor a owl:AnnotationProperty .
dcterms:author a owl:AnnotationProperty .
dcterms:license a owl:AnnotationProperty .
dc:publisher a owl:AnnotationProperty .


: a owl:Ontology ;
    dc:title "Thing Model Ontology"@en ;
    vann:preferredNamespacePrefix "tm" ;
    vann:preferredNamespaceUri "https://www.w3.org/2019/wot/tm#" ;
    owl:versionInfo "1.1.0" ;
    rdfs:comment "This ontology aims to model the Web of Things Thing Model according to the W3C Working Group (https://www.w3.org/WoT/)"@en ;
    dcterms:license <http://purl.org/NET/rdflicense/cc-by4.0> ;
    dcterms:contributor <https://vcharpenay.link/#me> ;
    dcterms:author "Mahda Noura (Siemens)" ;
    dcterms:author "Sebastian Kaebisch (Siemens)" ;
    dcterms:description "This ontology describes Thing Model concepts"@en ;
    dc:publisher [ a schema:Organization ; schema:name "W3C Web of Things Working Group"@en ; schema:url <https://www.w3.org/WoT/> ] .

:versionInfo rdf:type owl:AnnotationProperty ;
    rdfs:label "versionInfo" ;
    rdfs:comment "Provides version information of the TM ontology."@en ;
    rdfs:seeAlso schema:version ;
    rdfs:isDefinedBy tm: .

:ThingModel rdf:type rdfs:Class, owl:Class ;
    rdfs:label "ThingModel"@en ;
    rdfs:comment "A Thing Model is a description for a class of Things that have the same capabilities. It describes the Properties, Actions, and Events and common metadata that are shared for an entire group of Things. Compared to a Thing Description, a Thing Model does not contain enough information to identify or interact with a Thing instance."@en ;
    rdfs:isDefinedBy tm: .

:Version rdf:type rdfs:Class, owl:Class ;
    rdfs:label "Version"@en ;
    rdfs:comment "The Version is a container that provides versioning information for the Thing Model definition."@en ;
    rdfs:isDefinedBy tm: .

:hasVersion rdf:type owl:ObjectProperty ;
    rdfs:label "hasVersion" ;
    rdfs:comment "Relation between a Thing Model and the Version, that describes each Thing Model has a specific version."@en ;
    schema:domainIncludes :ThingModel ;
    schema:rangeIncludes :Version ;
    rdfs:isDefinedBy tm: .

:hasLink rdf:type owl:ObjectProperty ;
    rdfs:label "hasLink" ;
    rdfs:comment "Provides links to existing resources specified in a Thing Model to extend another Thing Model ."@en ;
    schema:domainIncludes :ThingModel ;
    schema:rangeIncludes hctl:Link ;
    rdfs:isDefinedBy tm: .

:model rdf:type owl:DatatypeProperty ;
    rdfs:label "model" ;
    rdfs:comment "Provides versioning information in the version container of a Thing Model."@en ;
    schema:domainIncludes :Version ;
    schema:rangeIncludes schema:Text ;
    rdfs:isDefinedBy tm: .

:title rdf:type owl:DatatypeProperty ;
    rdfs:label "title" ;
    rdfs:comment "Provide the title of the Thing Model elements (Thing, interaction affordance or data schema)" ;
    schema:domainIncludes :ThingModel ;
    schema:rangeIncludes schema:Text ;
    rdfs:subPropertyOf dcterms:title ;
    rdfs:isDefinedBy tm: .

:description rdf:type owl:DatatypeProperty ;
    rdfs:label "description" ;
    rdfs:comment "Provides description of the Thing Model element (Thing Model, interaction affordance, or data schema)" ;
    schema:domainIncludes :ThingModel ;
    schema:rangeIncludes schema:Text ;
    rdfs:subPropertyOf dcterms:description ;
    rdfs:isDefinedBy tm: .


:ref rdf:type owl:DatatypeProperty ;
    rdfs:label "ref" ;
    rdfs:comment "Provides a reference to an existing (external or local) definition that is copied into a newly defined definition. The reference value is based on three parts: an (optional) URI-reference (used for external reference), '#' sign, and JSON Pointer [RFC6901] value."@en ;
    rdfs:seeAlso schema:contactPoint ;
    rdfs:isDefinedBy : .

:required rdf:type owl:DatatypeProperty ;
    rdfs:label "required" ;
    rdfs:comment "Constraint that provides references to declarations in the Thing Model that are mandatory and must be present when Thing Description instances are derived from this Thing Model. The reference value is a JSON Pointer [RFC6901]."@en ;
    schema:domainIncludes :ThingModel ;
    schema:rangeIncludes schema:Text ;
    rdfs:isDefinedBy : .


:optional rdf:type owl:DatatypeProperty ;
    rdfs:label "optional" ;
    rdfs:comment "Constraint that provides references to declarations in the Thing Model that are optional and do not necessarily need to be implemented when Thing Description instances are derived from this Thing Model. The value of tm:optional MUST provide JSON Pointer [RFC6901] references to the required interaction model definitions."@en ;
    schema:domainIncludes :ThingModel ;
    schema:rangeIncludes schema:Text ;
    rdfs:isDefinedBy : .
