@prefix : <https://www.w3.org/2019/wot/tm#> .
@prefix dc: <http://purl.org/dc/elements/1.1/> .
@prefix owl: <http://www.w3.org/2002/07/owl#> .
@prefix rdf: <http://www.w3.org/1999/02/22-rdf-syntax-ns#> .
@prefix xml: <http://www.w3.org/XML/1998/namespace> .
@prefix xsd: <http://www.w3.org/2001/XMLSchema#> .
@prefix foaf: <http://xmlns.com/foaf/0.1/> .
@prefix rdfs: <http://www.w3.org/2000/01/rdf-schema#> .
@prefix vann: <http://purl.org/vocab/vann/> .
@prefix dcterms: <http://purl.org/dc/terms/> .
@prefix schema: <http://schema.org/> .
@prefix hctl: <https://www.w3.org/2019/wot/hypermedia#> .
@prefix tm: <https://www.w3.org/2019/wot/tm> .

: rdf:type owl:Ontology ;
    vann:preferredNamespacePrefix "tm" ;
    vann:preferredNamespaceUri "https://www.w3.org/2019/wot/tm#" ;
    owl:versionInfo "1.1.0" ;
    dc:title "Thing Model Ontology"@en ;
    rdfs:comment "This ontology aims to model the Web of Things domain according to the W3C Working Group (https://www.w3.org/WoT/)"@en ;
    dcterms:license <http://purl.org/NET/rdflicense/cc-by4.0> ;
    dcterms:contributor <https://vcharpenay.link/#me> ;
    dcterms:author "Mahda Noura (Siemens)" ;
    dcterms:author "Sebastian Kaebisch (Siemens)" ;
    dcterms:description "This ontology describes Thing Model concepts" ;
    dc:publisher [ a schema:Organization ; schema:name "W3C Web of Things Working Group"@en ; schema:url <https://www.w3.org/WoT/> ] .

:versionInfo rdf:type owl:AnnotationProperty ;
    rdfs:label "versionInfo" ;
    rdfs:comment "Provides version information."@en ;
    rdfs:seeAlso schema:version ;
    rdfs:isDefinedBy tm: .

:ThingModel rdf:type rdfs:Class, owl:Class ;
    rdfs:label "ThingModel"@en ;
    rdfs:comment "A Thing Model is a description for a class of Things that have the same capabilities. It describes the Properties, Actions, and Events and common metadata that are shared for an entire group of Things. Compared to a Thing Description, a Thing Model does not contain enough information to identify or interact with a Thing instance."@en ;
    rdfs:isDefinedBy tm: .

:Version rdf:type rdfs:Class, owl:Class ;
    rdfs:label "Version"@en ;
    rdfs:comment "The Version is a container that provides versioning information for the Thing Model definition."@en ;
    rdfs:isDefinedBy tm: .

:hasVersion rdf:type owl:ObjectProperty ;
    rdfs:label "hasVersion" ;
    rdfs:comment "Relation between a Thing Model and the Version, that describes each Thing Model has a specific version."@en ;
    schema:domainIncludes :ThingModel ;
    schema:rangeIncludes :Version ;
    rdfs:isDefinedBy tm: .

:hasLink rdf:type owl:ObjectProperty ;
    rdfs:label "hasLink" ;
    rdfs:comment "Provides links to existing resources specified in a Thing Model to extend another Thing Model ."@en ;
    schema:domainIncludes :ThingModel ;
    schema:rangeIncludes hctl:Link ;
    rdfs:isDefinedBy tm: .

:type rdf:type owl:DatatypeProperty ;
    rdfs:label "type" ;
    rdfs:comment "Indicates the type of the description."@en ;
    schema:domainIncludes :ThingModel ;
    schema:rangeIncludes schema:Text ; 
    rdfs:isDefinedBy tm: .

:model rdf:type owl:DatatypeProperty ;
    rdfs:label "model" ;
    rdfs:comment "Provides versioning information in the version container of a Thing Model."@en ;
    schema:domainIncludes :Version ;
    schema:rangeIncludes schema:Text ;
    rdfs:isDefinedBy tm: .

:title rdf:type owl:DatatypeProperty ;
    rdfs:label "title" ;
    rdfs:comment "title of the Thing Model element (Thing, interaction affordance or data schema)" ;
    schema:domainIncludes :ThingModel ;
    schema:rangeIncludes schema:Text ;
    rdfs:subPropertyOf dcterms:title ;
    rdfs:isDefinedBy tm: .

:description rdf:type owl:DatatypeProperty ;
    rdfs:label "description" ;
    rdfs:comment "description of the Thing Model element (Thing Model, interaction affordance, or data schema)" ;
    schema:domainIncludes :ThingModel ;
    schema:rangeIncludes schema:Text ;
    rdfs:subPropertyOf dcterms:description ;
    rdfs:isDefinedBy tm: .


